
% Compiler Design 3.9
\begin{exercise}{}
  Compute \(\nullable\), \(\first\), and \(\follow\) for the non-terminals \(A\)
  and \(B\) in the following grammar:
  %
  \begin{align*}
    A &::= BAa \\
    A &::=  \\
    B &::= bBc \\
    B &::= AA
  \end{align*}

  Remember to extend the language with an extra start production for the
  computation of \(\follow\).

  \begin{solution}
    \begin{enumerate}
      \item \(\nullable\): we get the constraints
      \begin{gather*}
        \nullable(A) = \nullable(BAa) \lor \nullable(\epsilon) \\
        \nullable(B) = \nullable(bBc) \lor \nullable(AA)
      \end{gather*}

      We can solve these to get \(\nullable(A) = \nullable(B) = true\).

      \item \(\first\): we get the constraints (given that both \(A\) and \(B\)
      are nullable):
      \begin{align*}
        \first(A) &= \first(BAa) \cup \first(\epsilon) \\
                  &= \first(B) \cup \first(A) \cup \emptyset \\
                  &= \first(B) \cup \first(A) \\
        \first(B) &= \first(bBc) \cup \first(AA) \\
                  &= \{b\} \cup \first(A) \cup \first(A) \cup \emptyset \\
                  &= \{b\} \cup \first(A)
      \end{align*}

      Starting from \(\first(A) = \first(B) = \emptyset\), we iteratively
      compute the fixpoint to get \(\first(A) = \first(B) = \{a, b\}\).

      \item \(\follow\): we add a production \(A' ::= A~\mathbf{EOF}\), and get
      the constraints (in order of productions):
      \begin{gather*}
        \{\mathbf{EOF}\} \subseteq \follow(A) \\
        \\
        \first(A) \subseteq \follow(B) \\
        \{a\} \subseteq \follow(A) \\
        \\
        \{c\} \subseteq \follow(B) \\
        \\
        \first(A) \subseteq \follow(A) \\
        \follow(B) \subseteq \follow(A)
      \end{gather*}

      Substituting the computed \(\first\) sets, and computing a fixpoint, we
      get \(\follow(A) = \{a, b, c,\mathbf{EOF}\}\) and \(\follow(B) = \{a, b,
      c\}\).
    \end{enumerate}
  \end{solution}
\end{exercise}

% Compiler design 3.11
\begin{exercise}{}
  
  Given the following grammar for arithmetic expressions:

  \begin{align*}
    S &::= Exp~\mathbf{EOF} \\
    Exp &::= Term~ Add \\
    Add &::= +~ Term~ Add \\
    Add &::= -~ Term~ Add \\
    Add &::= \\
    Term &::= Factor~ Mul \\
    Mul &::= *~ Factor~ Mul \\
    Mul &::= /~ Factor~ Mul \\
    Mul &::= \\
    Factor &::= \mathbf{num} \\
    Factor &::= (Exp) \\
  \end{align*}

  \begin{enumerate}
    \item Compute \(\nullable\), \(\first\), \(\follow\) for each of the
    non-terminals in the grammar.
    \item Check if the grammar is LL(1). If not, modify the grammar to make it
    so.
    \item Build the LL(1) parsing table for the grammar.
    \item Using your parsing table, parse or attempt to parse (till error) the
    following strings, assuming that \(\mathbf{num}\) matches any natural
    number:
    \begin{enumerate}
      \item \((3 + 4) * 5 ~\mathbf{EOF}\)
      \item \(2 + + ~\mathbf{EOF}\)
      \item \(2 ~\mathbf{EOF}\)
      \item \(2 * 3 + 4 ~\mathbf{EOF}\)
      \item \(2 + 3 * 4 ~\mathbf{EOF}\)
    \end{enumerate}
  \end{enumerate}

  \begin{solution}
    \begin{enumerate}
      \item We can compute the \(\nullable\), \(\first\), and \(\follow\) sets as:

        \begin{enumerate}
          \item \(\nullable\): 
          %
            \begin{align*}
              \nullable(S) &= false \\
              \nullable(Exp) &= false \\
              \nullable(Add) &= true \\
              \nullable(Term) &= false \\
              \nullable(Mul) &= true \\
              \nullable(Factor) &= false
            \end{align*}

          \item \(\first\): we have constraints:
            %
            \begin{align*}
              \first(S) &= \first(Exp) \\
              \first(Exp) &= \first(Term) \\
              \first(Add) &= \{+\} \cup \{-\} \cup \emptyset \\
              \first(Term) &= \first(Factor) \\
              \first(Mul) &= \{*\} \cup \{/\} \cup \emptyset \\
              \first(Factor) &= \{\mathbf{num}\} \cup \{(\}
            \end{align*}
            %
            which can be solved to get:
            %
            \begin{align*}
              \first(S) &= \{\mathbf{num}, (\} \\
              \first(Exp) &= \{\mathbf{num}, (\} \\
              \first(Add) &= \{+, -\} \\
              \first(Term) &= \{\mathbf{num}, (\} \\
              \first(Mul) &= \{*, /\} \\
              \first(Factor) &= \{\mathbf{num}, (\}
            \end{align*}
          \item \(\follow\): we have constraints (for each rule, except
          empty/terminal rules):
          \begin{multicols}{2}
            \allowdisplaybreaks
            \begin{align*}
              \{\mathbf{EOF}\} &\subseteq \follow(Exp) \\
              &\\
              \first(Add) &\subseteq \follow(Term) \\
              \follow(Exp) &\subseteq \follow(Term) \\
              \follow(Exp) &\subseteq \follow(Add) \\
              &\\
              \first(Add) &\subseteq \follow(Term) \\
              \follow(Add) &\subseteq \follow(Term) \\
              &\\
              \first(Add) &\subseteq \follow(Term) \\
              \follow(Add) &\subseteq \follow(Term) \\
              &\\
              \first(Mul) &\subseteq \follow(Factor) \\
              \follow(Term) &\subseteq \follow(Factor) \\
              \follow(Term) &\subseteq \follow(Mul) \\
              &\\
              \first(Mul) &\subseteq \follow(Factor) \\
              \follow(Mul) &\subseteq \follow(Factor) \\
              &\\
              \first(Mul) &\subseteq \follow(Factor) \\
              \follow(Mul) &\subseteq \follow(Factor) \\
              &\\
              \{)\} &\subseteq \follow(Exp) \\
            \end{align*}
          \end{multicols}

          The fixpoint can again be computed to get:
          \begin{align*}
            \follow(S) &= \{\} \\
            \follow(Exp) &= \{), \mathbf{EOF}\} \\
            \follow(Add) &= \{), \mathbf{EOF}\} \\
            \follow(Term) &= \{+, -, ), \mathbf{EOF}\} \\
            \follow(Mul) &= \{+, -, ), \mathbf{EOF}\} \\
            \follow(Factor) &= \{+, -, *, /, ), \mathbf{EOF}\}
          \end{align*}

        \end{enumerate}
      \item The grammar is LL(1), there are no conflicts. Demonstrated by the
      parsing table below.
      \item LL(1) parsing table:
        \begin{center}
          \begin{tabular}{c|c|c|c|c|c|c|c|c}
            & \(\mathbf{num}\) & \(+\) & \(-\) & \(*\) & \(/\) & \((\) & \()\) & \(\mathbf{EOF}\) \\
            \hline
            \(S\) & 1 & & & & & 1 & &\\
            \(Exp\) & 1 & & & & & 1 & &\\
            \(Add\) & & 1 & 2 & & & & 3 & 3 \\
            \(Term\) & 1 & & & & & 1 & & \\
            \(Mul\) & & 3 & 3 & 1 & 2 & & 3 & 3 \\
            \(Factor\) & 1 & & & & & 2 & & \\
          \end{tabular}
        \end{center}
      \item Parsing the strings:
      \begin{enumerate}
        \item \((3 + 4) * 5 ~\mathbf{EOF}\) \checkmark
        \item \(2 + + ~\mathbf{EOF}\) --- fails on the second \(+\). The
        corresponding error cell in the parsing table is \((Term, +)\).
        \item \(2 ~\mathbf{EOF}\) \checkmark
        \item \(2 * 3 + 4 ~\mathbf{EOF}\) \checkmark
        \item \(2 + 3 * 4 ~\mathbf{EOF}\) \checkmark
      \end{enumerate}

      Example step-by-step LL(1) parsing state for \(2 * 3 + 4\):
      \begin{center}
        \begin{tabular}{c c c}
          Lookahead & Stack & Next Rule \\
          \hline
          \(2\) & \(S\) & \(S ::= Exp ~\mathbf{EOF}\)\\
          \(2\) & \(Exp ~ \mathbf{EOF}\) & \(Exp ::= Term~Add\)\\
          \(2\) & \(Term ~ Add ~ \mathbf{EOF}\) & \(Term ::= Factor~Mul\)\\
          \(2\) & \(Factor ~ Mul ~ Add ~ \mathbf{EOF}\) & \(Factor ::= \mathbf{num}\)\\
          \(2\) & \(\mathbf{num} ~ Mul ~ Add ~ \mathbf{EOF}\) & \(match(\mathbf{num})\)\\
          \(*\) & \(Mul ~ Add ~ \mathbf{EOF}\) & \(Mul ::= *~Factor~Mul\)\\
          \(*\) & \(* ~Factor ~ Mul ~ Add ~ \mathbf{EOF}\) & \(match(*)\)\\
          \(3\) & \(Factor ~ Mul ~ Add ~ \mathbf{EOF}\) & \(Factor ::= \mathbf{num}\)\\
          \(3\) & \(\mathbf{num} ~ Mul ~ Add ~ \mathbf{EOF}\) & \(match(\mathbf{num})\)\\
          \(+\) & \(Mul ~ Add ~ \mathbf{EOF}\) & \(Mul ::=\)\\
          \(+\) & \(Add ~ \mathbf{EOF}\) & \(Add ::= +~Term~Add\)\\
          \(+\) & \(+ ~Term ~Add ~ \mathbf{EOF}\) & \(match(+)\)\\
          \(4\) & \(Term ~Add ~ \mathbf{EOF}\) & \(Term ::= Factor~Term*\)\\
          \(4\) & \(Factor ~Mul ~Add ~ \mathbf{EOF}\) & \(Factor ::= \mathbf{num}\)\\
          \(4\) & \(\mathbf{num} ~Mul ~Add ~ \mathbf{EOF}\) & \(match(\mathbf{num})\)\\
          \(\mathbf{EOF}\) & \(Mul ~Add ~ \mathbf{EOF}\) & \(Mul ::= \)\\
          \(\mathbf{EOF}\) & \(Add ~ \mathbf{EOF}\) & \(Add ::= \)\\
          \(\mathbf{EOF}\) & \(\mathbf{EOF}\) & \(match(\mathbf{EOF})\)\\
        \end{tabular}
      \end{center}
    \end{enumerate}
  \end{solution}

\end{exercise}

